coqimp/contextswitch/proof/SaveUsedWindows.v
@@ -1,0 +1,389 @@
+Require Import Coqlib.                                                    
+Require Import Maps.            
+Require Import LibTactics.   
+        
+Require Import Integers.  
+Open Scope Z_scope.        
+Import ListNotations.  
+   
+Set Asymmetric Patterns.  
+        
+Require Import state.    
+Require Import language.  
+ 
+Set Implicit Arguments.    
+Unset Strict Implicit. 
+               
+Require Import logic.
+    
+Require Import lemmas.
+Require Import lemmas_ins.
+
+Require Import Coq.Logic.FunctionalExtensionality.
+
+Require Import integer_lemma.
+
+Require Import sep_lemma.
+Require Import reg_lemma.
+Require Import derived_rule.
+
+Require Import tm_dly_lemma.
+
+Require Import code.
+Require Import ctxswitch_spec.
+
+Require Import lemma1.
+
+Open Scope nat.
+Open Scope code_scope.
+Open Scope mem_scope.
+
+(*+ Lemmas +*)
+Ltac solve_element_vi vi :=
+  match goal with
+  | H : vi = _ \/ _ |- _ =>
+    destruct H as [?a | H]; [subst; tryfalse; eauto | solve_element_vi vi]
+  | H : vi = _ |- _ =>
+    subst; tryfalse; eauto
+  | _ => idtac
+  end.
+
+Ltac solve_element_id id vi :=
+  match goal with
+  | H : id = _ \/ _ |- _ =>
+    destruct H as [?a | H];
+    [subst; solve_element_vi vi | solve_element_id id vi]
+  | H : id = _ |- _ =>
+    subst; solve_element_vi vi
+  | _ => idtac
+  end.
+
+Lemma post_cons_neq_still :
+  forall id vi,
+    $ 0 <=ᵤᵢ id <=ᵤᵢ $ 7 -> $ 0 <=ᵤᵢ vi <=ᵤᵢ $ 7 ->
+    id <> post_cwp vi ->
+    post_cwp id <> post_cwp (post_cwp vi).
+Proof.
+  intros.
+  intro.
+  eapply H1.
+  unfolds post_cwp.
+  eapply in_range_0_7_num in H.
+  eapply in_range_0_7_num in H0.
+  unfolds N.
+  solve_element_id id vi.
+Qed.
+
+Lemma post_cons_neq_still_rev :
+  forall id vi,
+    post_cwp id <> post_cwp (post_cwp vi) ->
+    id <> post_cwp vi.
+Proof.
+  intros.
+  intro.
+  eapply H.
+  subst; eauto.
+Qed.
+
+Lemma post_1_neq' :
+  forall id,
+    $ 0 <=ᵤᵢ id <=ᵤᵢ $ 7 ->
+    id <> post_cwp id.
+Proof.
+  intros.
+  intro.
+  symmetry in H0.
+  eapply post_1_neq in H0; eauto.
+Qed.
+
+Lemma stack_frame_match_fm_save :
+  forall fm F oid id cl clfp1 clfp2,
+    $ 0 <=ᵤᵢ oid <=ᵤᵢ $ 7 -> $ 0 <=ᵤᵢ id <=ᵤᵢ $ 7 ->
+    stack_frame_match oid clfp1 (F ++ fm :: nil) id -> length F = 13 ->
+    stack_frame_save (F ++ fm :: nil) (cl, clfp1 ++ clfp2)
+                     (cl, clfp1 ++ clfp2) oid (post_cwp id).
+Proof.
+  intros.
+  unfold stack_frame_save.
+  split; eauto.
+  do 14 (try destruct F; simpl in H2; tryfalse).
+  simpl in H1.
+  
+  inversion H1; subst.
+  {
+    simpl.
+    eapply frame_save_end; eauto.
+  }
+
+  inversion H10; subst.
+  {
+    simpl. 
+    eapply frame_save_cons; eauto.
+    eapply post_cons_neq_still; eauto.
+    eapply frame_save_end; eauto.
+  }
+
+  Ltac solve_post_inrange :=
+    match goal with
+    | |- $ 0 <=ᵤᵢ (post_cwp _) <=ᵤᵢ $ 7 =>
+      eapply in_range_0_7_post_cwp_still; solve_post_inrange
+    | _ => eauto
+    end.
+
+  Ltac solve_post_neq :=
+    match goal with
+    | |- post_cwp _ <> post_cwp (post_cwp _) =>
+      eapply post_cons_neq_still;
+      [solve_post_inrange | solve_post_inrange | solve_post_neq]
+    | |- ?id <> post_cwp ?id =>
+      eapply post_1_neq'; solve_post_inrange
+    | _ => eauto
+    end.
+  
+  inversion H12; subst.
+  {
+    simpl. 
+    do 2 (eapply frame_save_cons; [solve_post_neq | idtac]).
+    eapply frame_save_end; eauto.
+  }
+  
+  inversion H14; subst.
+  {
+    simpl.
+    do 2 (eapply frame_save_cons; [solve_post_neq | idtac]).
+    eapply post_cons_neq_still_rev; eauto.
+    eapply frame_save_cons; [solve_post_neq | idtac].
+    eapply frame_save_end; eauto.
+  }
+  
+  inversion H16; subst.
+  {
+    simpl.
+    do 3 (eapply frame_save_cons; [solve_post_neq | idtac];
+          try eapply post_cons_neq_still_rev; eauto).
+    eapply post_cons_neq_still_rev; eauto.
+    eapply frame_save_cons; [solve_post_neq | idtac].
+    eapply frame_save_end; eauto.
+  }
+
+  inversion H18; subst.
+  {
+    simpl.
+    do 4 (eapply frame_save_cons; [solve_post_neq | idtac];
+          do 2 (try eapply post_cons_neq_still_rev; eauto)).
+    eapply post_cons_neq_still_rev; eauto.
+    eapply frame_save_cons; [solve_post_neq | idtac];
+      do 2 (try eapply post_cons_neq_still_rev; eauto).
+    eapply frame_save_end; eauto.
+  }
+
+  inversion H20; subst.
+  {
+    simpl.
+    do 6 (try eapply frame_save_cons; [solve_post_neq | idtac];
+          repeat (eapply post_cons_neq_still_rev; eauto)).
+    eapply frame_save_end; eauto.
+  }
+
+  inversion H22; subst.
+  {
+    simpl.
+    do 7 (try eapply frame_save_cons; [solve_post_neq | idtac];
+          repeat (eapply post_cons_neq_still_rev; eauto)).
+    eapply frame_save_end; eauto.
+  }
+Qed.
+  
+(*+ Proof +*)
+Theorem Ta0SaveUsedWindowsProof :
+  forall vl,
+    spec |- {{ ta0_save_usedwindows_pre vl }}
+             ta0_save_usedwindows
+           {{ ta0_save_usedwindows_post vl }}.
+Proof.
+  intros.
+  unfold ta0_save_usedwindows_pre.
+  unfold ta0_save_usedwindows_post.
+  hoare_ex_intro_pre. 
+  renames x'0 to fmg', x'2 to fmo', x'4 to fml', x'6 to fmi'.
+  renames x'8 to id, x'12 to vi, x'10 to F', x'11 to vy.
+  renames x'23 to vz, x'24 to vn, x'15 to ct, x'20 to nt, x'13 to ll.
+  renames x'16 to cctx, x'17 to cl, x'18 to clfp1, x'19 to clfp2.
+  renames x'21 to nctx, x'22 to nstk.
+  renames x'7 to oid, x'1 to fmo, x'3 to fml, x'5 to fmi, x'9 to F, x'14 to i.
+
+  eapply Pure_intro_rule.
+  introv Hlgvl.
+  hoare_lift_pre 15.
+  eapply Pure_intro_rule.
+  introv Hnctx.
+  hoare_lift_pre 15.
+  eapply Pure_intro_rule.
+  introv Hstk_fm_match.
+  hoare_lift_pre 15.
+  eapply Pure_intro_rule.
+  introv Hfm_restore.
+  hoare_lift_pre 15.
+  eapply Pure_intro_rule.
+  introv Hstk_fm_constraint.
+  hoare_lift_pre 15.
+  eapply Pure_intro_rule.
+  introv Hg4.
+  destruct Hg4 as [Hg4 [Hrot [Hoid_range [Hg4_vl Hg7] ] ] ].
+  hoare_lift_pre 15.
+  eapply Pure_intro_rule.
+  introv Hctx_win_save.
+  
+  unfold ta0_save_usedwindows.
+ 
+  destruct fmg', fmo', fml', fmi'.
+  
+  (** sll g4 1 g5 *)
+  hoare_lift_pre 2.
+  eapply backward_rule.
+  introv Hs.
+  eapply Regs_Global_combine_GenRegs in Hs; eauto.
+  eapply seq_rule; eauto.
+  TimReduce_simpl.
+  eapply sll_rule_reg; eauto.
+  simpl; eauto.
+  rewrite in_range1; eauto.
+  simpl upd_genreg.
+  rewrite get_range_0_4_stable; eauto.
+
+  (** srl g4 (OS_WINDOWS - 1) g4 *)
+  unfold OS_WINDOWS.
+  assert (Heq7 : ($ 8) -ᵢ ($ 1) = ($ 7)).
+  eauto.
+  rewrite Heq7; eauto.
+  eapply seq_rule; eauto.
+  TimReduce_simpl.
+  eapply srl_rule_reg; eauto.
+  simpl; eauto.
+  rewrite in_range7; eauto.
+  simpl upd_genreg.
+  
+  simpl in Hg4.
+  inversion Hg4; subst.
+  rewrite get_range_0_4_stable; eauto.
+
+  (** or g4 g5 g4 *)
+  eapply seq_rule.
+  TimReduce_simpl.
+  eapply or_rule_reg; eauto.
+  simpl; eauto.
+  simpl upd_genreg.
+
+  (** andcc g4 g7 g0 *)
+  hoare_lift_pre 4.
+  hoare_lift_pre 5.
+  hoare_lift_pre 3.
+  eapply seq_rule; eauto.
+  TimReduce_simpl.
+  eapply andcc_rule_reg; eauto.
+  simpl; eauto.
+  simpl upd_genreg.
+  simpl get_genreg_val; eauto.
+
+  (** bne Ta0_Task_Switch_NewContext; nop *)
+  simpl in Hg7.
+  destruct Hg7 as [Hg7 Hct_not_null].
+  inversion Hg7; subst.
+  eapply hoare_pure_gen' with (pu := $ 0 <=ᵤᵢ id <=ᵤᵢ $ 7 /\ $ 0 <=ᵤᵢ vi <=ᵤᵢ $ 7).
+  {
+    introv Hs.
+    simpl_sep_liftn_in Hs 4.
+    unfold FrameState in Hs.
+    asrt_to_line_in Hs 3.
+    simpl_sep_liftn_in Hs 4.
+    eapply sep_pure_l_elim in Hs; eauto.
+    simpljoin1; eauto.
+  }
+  eapply Pure_intro_rule.
+  introv Hid_inrange.
+  destruct Hid_inrange as [Hid_inrange Hvi_inrange].
+  
+  assert (Hiszero : iszero ((i >>ᵢ ($ 7)) |ᵢ (i <<ᵢ ($ 1))) &ᵢ (($ 1) <<ᵢ vi) =
+          iszero (get_range 0 7 (i >>ᵢ ($ 7)) |ᵢ (i <<ᵢ ($ 1))) &ᵢ (($ 1) <<ᵢ vi)).
+  {
+    rewrite in_range_0_7_and; eauto.
+  }
+  rewrite Hiszero.
+  rewrite g4_val_get_range_0_7_equal with (id := id); eauto.
+  
+  eapply Bne_rule; eauto.
+  {
+    eval_spec.
+  }
+  {
+    TimReduce_simpl.
+    eapply nop_rule; eauto.
+  }
+  {
+    TimReduce_simpl.
+    introv Hs.
+    sep_cancel1 3 1.
+    simpl; eauto.
+  }
+
+  Focus 3.
+  introv Hnxt_invalid.
+  unfold iszero in Hnxt_invalid.
+  destruct (Int.eq_dec (($ 1) <<ᵢ (post_cwp id)) &ᵢ (($ 1) <<ᵢ vi) $ 0); tryfalse.
+  clear Hnxt_invalid.
+  renames n to Hnxt_invalid.
+  eapply and_not_zero_eq in Hnxt_invalid; eauto.
+
+  split.
+  
+    introv Hs.
+    unfold ta0_task_switch_newcontext_pre.
+    sep_ex_intro.
+    asrt_to_line 14.
+    eapply sep_pure_l_intro; eauto.
+    simpl_sep_liftn 2.
+    eapply GenRegs_split_Regs_Global.
+    sep_cancel1 1 1.
+    sep_cancel1 3 1.
+    sep_cancel1 3 1.
+    sep_cancel1 1 2.
+    do 5 sep_cancel1 1 1.
+    sep_cancel1 3 1.
+    sep_cancel1 3 1.
+    eapply sep_pure_l_intro; eauto.
+    eapply sep_pure_l_intro; eauto.
+
+    introv Hs.
+    unfold ta0_task_switch_newcontext_post in Hs.
+    sep_ex_elim_in Hs.
+    asrt_to_line_in Hs 13.
+    eapply sep_pure_l_elim in Hs.
+    destruct Hs as [Hlgvl1 Hs].
+    symmetry in Hlgvl1.
+    inversion Hlgvl1; subst.
+    sep_ex_intro.  
+    eapply sep_pure_l_intro; eauto. 
+    do 10 sep_cancel1 1 1.
+    sep_cancel1 4 1.
+    sep_cancel1 4 1.
+    eapply sep_pure_l_intro; eauto.
+    do 2 sep_cancel1 1 1.
+    sep_cancel1 1 2.
+    instantiate (1 := Aemp).
+    eapply astar_emp_intro_r; eauto.
+    eapply sep_pure_l_intro; eauto.
+    introv Hct.
+    destruct Hctx_win_save as [Hctx_win_save Hctx_pt_stk].
+    split; eauto.
+    split; eauto.
+    Print stack_frame_save.
+    instantiate (1 := (post_cwp id)).
+    instantiate (1 := oid).
+    instantiate (2 := F).
+    instantiate (1 := fmo). 
+    eapply stack_frame_match_fm_save; eauto.
+    simpljoin1; eauto.
+    simpljoin1; eauto.
+    eapply in_range_0_7_post_cwp_still; eauto.
+
+  introv Hnjp.
